Add JSON normalization, proof progress for unary operators, bug fixes in ImpQcert to ImpJson translation
Signed-off-by: Jerome Simeon <jeromesimeon@me.com>

coq/Utils/Bindings.v
@@ -21,6 +21,7 @@ Bindings are used as a representation for records and environments. *)
 
 
 Require Import List.
+Require Import ListSet.
 Require Import Sumbool.
 Require Import Arith.
 Require Import Bool.
@@ -1956,5 +1957,313 @@ Section MergeBindings.
 
 End MergeBindings.
 
-Hint Resolve @merge_bindings_sorted.
+Section RecProject.
+  Import ListNotations.
+  Definition rproject {A} (l:list (string*A)) (s:list string) : list (string*A) :=
+    filter (fun x => if in_dec string_dec (fst x) s then true else false) l.
 
+  Lemma rproject_nil_l {A} (s:list string) :
+    @rproject A [] s = [].
+  Proof.
+    reflexivity.
+  Qed.
+
+  Lemma rproject_nil_r {A} (l:list (string*A)) :
+    @rproject A l [] = [].
+  Proof.
+    induction l. reflexivity.
+    simpl. apply IHl.
+  Qed.
+
+  Lemma rproject_rec_sort_commute {B} (l1:list (string*B)) sl:
+    rproject (rec_sort l1) sl = rec_sort (rproject l1 sl).
+  Proof.
+    unfold rproject.
+    apply rec_sort_filter_fst_commute; intros.
+    simpl.
+    match_destr.
+  Qed.
+
+  Lemma rproject_map_fst_same {B C} (f:string*B->string*C) (l:list (string*B)) sl
+        (samedom:forall a, In a l -> fst (f a) = fst a) :
+    rproject (map f l) sl = map f (rproject l sl).
+  Proof.
+    induction l; simpl; trivial.
+    simpl in samedom.
+    destruct (in_dec string_dec (fst (f a)) sl);
+      destruct (in_dec string_dec (fst a) sl).
+    - rewrite IHl; intuition.
+    - rewrite samedom in i; intuition.
+    - rewrite <- samedom in i; intuition.
+    - rewrite IHl; intuition.
+  Qed.
+
+  Lemma rproject_app {B} (l1 l2:list (string*B)) sl:
+    rproject (l1 ++ l2) sl = (rproject l1 sl) ++ (rproject l2 sl).
+  Proof.
+    unfold rproject.
+    apply filter_app.
+  Qed.
+
+  Lemma rproject_rproject  {B} (l:list (string*B)) sl1 sl2:
+    rproject (rproject l sl2) sl1 = rproject l (set_inter string_dec sl2 sl1).
+  Proof.
+    unfold rproject.
+    rewrite filter_and; simpl.
+    apply filter_ext; intros.
+    repeat match_destr; simpl; trivial.
+    - specialize (set_inter_intro string_dec (fst x) sl2 sl1); intuition.
+    - specialize (set_inter_elim1 string_dec (fst x) sl2 sl1); intuition.
+    - specialize (set_inter_elim2 string_dec (fst x) sl2 sl1); intuition.
+    - apply set_inter_elim in i; intuition.
+  Qed.
+
+  Lemma rproject_Forall2_same_domain {B C} P (l1:list(string*B)) (l2:list (string*C)) ls :
+    Forall2 P l1 l2 ->
+    domain l1 = domain l2 ->
+    Forall2 P (rproject l1 ls) (rproject l2 ls).
+  Proof.
+    unfold rproject; intros.
+    apply filter_Forall2_same; trivial.
+    revert H0; clear. revert l2.
+    induction l1; destruct l2; simpl; trivial; try discriminate.
+    inversion 1.
+    rewrite H1.
+    match_destr; f_equal; auto.
+  Qed.
+
+  Lemma sublist_rproject {A} (l:list(string*A)) sl: sublist (rproject l sl) l.
+  Proof.
+    induction l; simpl.
+    - constructor.
+    - match_destr.
+      + apply sublist_cons; auto.
+      + apply sublist_skip; auto.
+  Qed.
+
+  Lemma rproject_remove_all {B} s sl (l1:list(string*B)):
+    rproject l1 (remove_all s sl) =
+    filter (fun x => nequiv_decb s (fst x)) (rproject l1 sl).
+  Proof.
+    rewrite remove_all_filter.
+    induction l1; simpl; trivial.
+    rewrite IHl1.
+    destruct (in_dec string_dec (fst a) sl); destruct (in_dec string_dec (fst a) (filter (nequiv_decb s) sl)); simpl.
+    - apply filter_In in i0. destruct i0 as [inn neq].
+      rewrite neq; trivial.
+    - match_case; intros eqq.
+      elim n. apply filter_In; intuition.
+    - apply filter_In in i; intuition.
+    - trivial.
+  Qed.
+
+  Lemma rec_sort_rproject_remove_all_in {B} s sl l1 l2 :
+    In s sl ->
+    In s (@domain _ B l2) -> 
+    rec_sort (rproject l1 sl ++ l2) = 
+    rec_sort (rproject l1 (remove_all s sl) ++ l2).
+  Proof.
+    intros.
+    rewrite rproject_remove_all.
+    rewrite (rec_sort_filter_latter_from_former s); trivial.
+  Qed.
+
+  Lemma rec_sort_rproject_remove_in {B} s sl l1 l2 :
+    In s sl ->
+    In s (@domain _ B l2) -> 
+    rec_sort (rproject l1 sl ++ l2) = 
+    rec_sort (rproject l1 (remove string_dec s sl) ++ l2).
+  Proof.
+    intros.
+    rewrite (rec_sort_rproject_remove_all_in s); trivial.
+  Qed.
+
+  Lemma rproject_with_lookup {A} (l1 l2:list (string * A)) (s:list string):
+    is_list_sorted ODT_lt_dec (domain l1) = true ->
+    is_list_sorted ODT_lt_dec (domain l2) = true ->
+    sublist l1 l2 ->
+    (forall x, In x s -> assoc_lookupr string_dec l1 x = assoc_lookupr string_dec l2 x) ->
+    rproject l1 s = rproject l2 s.
+  Proof.
+    intros.
+    revert l1 H H1 H2; induction l2; simpl; intros.
+    - apply sublist_nil_r in H1; subst; simpl; auto 1.
+    - destruct a.
+      simpl.
+      assert (is_list_sorted ODT_lt_dec (domain l2) = true)
+        by (apply (@rec_sorted_skip_first string ODT_string _ l2 (s0,a)); assumption).
+      specialize (IHl2 H3).
+      assert (NoDup (domain ((s0,a)::l2)))
+        by (apply is_list_sorted_NoDup_strlt; assumption).
+      generalize (sublist_cons_inv' H1 H4); intros.
+      elim H5; clear H5; intros.
+      + elim H5; clear H5; intros.
+        elim H5; clear H5; intros.
+        rewrite H5 in *.
+        assert (is_list_sorted ODT_lt_dec (domain x) = true)
+          by (apply (@rec_sorted_skip_first string ODT_string _  x (s0,a)); assumption).
+        simpl.
+        specialize (IHl2 x H7 H6).
+        simpl in H2.
+        rewrite IHl2; try reflexivity; intros.
+        simpl in H2.
+        case_eq (string_dec x0 s0); intros.
+        * subst.
+          assert (NoDup (domain ((s0,a)::x))) by (apply is_list_sorted_NoDup_strlt; assumption).
+          assert (assoc_lookupr string_dec x s0 = None) by
+              (apply assoc_lookupr_nin_none; inversion H5; assumption).
+          assert (assoc_lookupr string_dec l2 s0 = None) by
+              (apply assoc_lookupr_nin_none; inversion H4; assumption).
+          rewrite H10; rewrite H11; reflexivity.
+        * specialize (H2 x0 H8).
+          destruct(string_dec x0 s0) ; try congruence.
+          destruct (assoc_lookupr string_dec x x0);
+            destruct (assoc_lookupr string_dec l2 x0); try congruence.
+      + elim H5; clear H5; intros.
+        case_eq (in_dec string_dec s0 s); intros.
+        specialize (H2 s0 i).
+        destruct (string_dec s0 s0); try congruence.
+        simpl in H5.
+        assert (assoc_lookupr string_dec l1 s0 = None)
+          by (apply assoc_lookupr_nin_none; assumption).
+        rewrite H8 in *.
+        destruct (assoc_lookupr string_dec l2 s0); congruence.
+        rewrite (IHl2 l1 H H6); try reflexivity; intros.
+        specialize (H2 x H8).
+        case_eq (string_dec x s0); intros; subst.
+        congruence.
+        rewrite H9 in *.
+        destruct (assoc_lookupr string_dec l1 x); destruct (assoc_lookupr string_dec l2 x); try congruence.
+  Qed.
+
+  Lemma rproject_sublist {A} (l1 l2:list (string * A)) (s:list string) :
+    is_list_sorted ODT_lt_dec (domain l1) = true ->
+    is_list_sorted ODT_lt_dec (domain l2) = true ->
+    sublist s (domain l1) ->
+    sublist l1 l2 ->
+    rproject l1 s = rproject l2 s.
+  Proof.
+    intros.
+    assert (sublist s (domain l2))
+      by (apply (sublist_trans s (domain l1) (domain l2)); try assumption;
+          apply sublist_domain; assumption).
+    apply rproject_with_lookup; try assumption; intros.
+    assert (In x (domain l1)) by (apply (sublist_In H1); assumption).
+    assert (In x (domain l2)) by (apply (sublist_In H3); assumption).
+    generalize (in_dom_lookupr l1 x string_dec); intros.
+    elim (H7 H5); intros.
+    assert (assoc_lookupr string_dec l2 x = Some x0).
+    assert (NoDup (domain l2)) by (apply is_list_sorted_NoDup_strlt; assumption).
+    apply (assoc_lookupr_nodup_sublist H9 H2); assumption.
+    rewrite H8; rewrite H9; reflexivity.
+  Qed.
+
+  Lemma rproject_equivlist {B} (l:list (string*B)) sl1 sl2 :
+    equivlist sl1 sl2 ->
+    rproject l sl1 = rproject l sl2.
+  Proof.
+    induction l; simpl; trivial.
+    intros eqq.
+    rewrite (IHl eqq).
+    destruct (in_dec string_dec (fst a) sl1);
+      destruct (in_dec string_dec (fst a) sl2); trivial.
+    - apply eqq in i; intuition.
+    - apply eqq in i; intuition.
+  Qed.
+
+  Lemma rproject_sortfilter {B} (l:list (string*B)) sl1 :
+    rproject l (insertion_sort ODT_lt_dec sl1) = rproject l sl1.
+  Proof.
+    apply rproject_equivlist.
+    apply insertion_sort_trich_equiv.
+    apply StringOrder.trichotemy.
+  Qed.
+
+  Lemma rproject_concat_dist {A} (l1 l2:list (string * A)) (s:list string) :
+    rproject (rec_concat_sort l1 l2) s = rec_concat_sort (rproject l1 s) (rproject l2 s).
+  Proof.
+    unfold rec_concat_sort.
+    rewrite rproject_rec_sort_commute.
+    rewrite rproject_app.
+    reflexivity.
+  Qed.
+
+  Lemma rproject_domain_in {A} s (l1:list (string*A)) l2 :
+    In s (domain l1) /\ In s l2 <->
+    In s (domain (rproject l1 l2)).
+  Proof.
+    split; intros.
+    - destruct H as [inn1 inn2].
+      unfold rproject.
+      apply in_domain_in in inn1.
+      destruct inn1 as [x inn1].
+      apply (in_dom (b:=x)).
+      apply filter_In; split; trivial; simpl.
+      match_destr.
+      tauto.
+    - apply in_domain_in in H.
+      destruct H as [x inn].
+      unfold rproject in inn.
+      apply filter_In in inn.
+      simpl in inn.
+      destruct inn as [inn1 inn2].
+      match_destr_in inn2.
+      split; trivial.
+      eapply in_dom; eauto.
+  Qed.
+
+End RecProject.
+
+Section RecRemove.
+  Definition rremove {A} (l:list (string*A)) (s:string) : list (string*A) :=
+    filter (fun x => if string_dec s (fst x) then false else true) l.
+
+  Lemma is_sorted_rremove {A} (l:list (string * A)) (s:string):
+    is_list_sorted ODT_lt_dec (domain l) = true ->
+    is_list_sorted ODT_lt_dec (domain (rremove l s)) = true.
+  Proof.
+    unfold rremove; intros.
+    apply (@sorted_over_filter string ODT_string); assumption.
+  Qed.
+
+  Lemma domain_rremove {A} s (l:list (string*A)) :
+    domain (rremove l s) = remove_all s (domain l).
+  Proof.
+    induction l; simpl; trivial.
+    unfold equiv_dec, string_eqdec.
+    destruct (string_dec s (fst a)); simpl; trivial.
+    f_equal; trivial.
+  Qed.
+
+  Lemma rremove_rec_sort_commute {B} (l1:list (string*B)) s:
+    rremove (rec_sort l1) s = rec_sort (rremove l1 s).
+  Proof.
+    unfold rremove.
+    apply rec_sort_filter_fst_commute; intros.
+    simpl.
+    match_destr.
+  Qed.
+
+  Lemma rremove_app {B} (l1 l2:list (string*B)) s:
+    rremove (l1 ++ l2) s = rremove l1 s ++ rremove l2 s.
+  Proof.
+    unfold rremove.
+    apply filter_app.
+  Qed.
+
+  Lemma nin_rremove {B} (l:list (string*B)) s :
+    ~ In s (domain l) ->
+    rremove l s = l.
+  Proof.
+    intros nin.
+    apply true_filter; intros ? inn.
+    destruct x.
+    apply in_dom in inn.
+    simpl.
+    match_destr.
+    congruence.
+  Qed.
+
+End RecRemove.
+
+Hint Resolve @merge_bindings_sorted.
