coq/Utils/JSONNorm.v
@@ -1,0 +1,217 @@
+(*
+ * Copyright 2015-2016 IBM Corporation
+ *
+ * Licensed under the Apache License, Version 2.0 (the "License");
+ * you may not use this file except in compliance with the License.
+ * You may obtain a copy of the License at
+ *
+ * http://www.apache.org/licenses/LICENSE-2.0
+ *
+ * Unless required by applicable law or agreed to in writing, software
+ * distributed under the License is distributed on an "AS IS" BASIS,
+ * WITHOUT WARRANTIES OR CONDITIONS OF ANY KIND, either express or implied.
+ * See the License for the specific language governing permissions and
+ * limitations under the License.
+ *)
+
+Require Import String.
+Require Import List.
+Require Import Sumbool.
+Require Import Arith.
+Require Import Bool.
+Require Import EquivDec.
+Require Import Assoc.
+Require Import Bindings.
+Require Import SortingAdd.
+Require Import CoqLibAdd.
+Require Import JSON.
+
+Section JSONNorm.
+  Fixpoint normalize_json (d:json) : json :=
+    match d with
+    | jobject rl => jobject (rec_sort (map (fun x => (fst x, normalize_json (snd x))) rl))
+    | jarray l => jarray (map normalize_json l)
+    | _ => d
+    end.
+
+  Inductive json_normalized : json -> Prop :=
+  | jnnull :
+      json_normalized jnull
+  | jnnumber n :
+      json_normalized (jnumber n)
+  | jnbool b :
+      json_normalized (jbool b)
+  | jnstring s :
+      json_normalized (jstring s)
+  | jnarray dl :
+      Forall (fun x => json_normalized x) dl -> json_normalized (jarray dl)
+  | jnobject dl :
+      Forall (fun d => json_normalized (snd d)) dl ->
+      (is_list_sorted ODT_lt_dec (domain dl) = true) ->
+      json_normalized (jobject dl).
+
+  Theorem normalize_normalizes :
+    forall (d:json), json_normalized (normalize_json d).
+  Proof.
+    induction d using jsonInd2; simpl.
+    - apply jnnull.
+    - apply jnnumber.
+    - apply jnbool.
+    - apply jnstring.
+    - apply jnarray.
+      apply Forall_forall; intros.
+      induction c; elim H0; intros.
+      rewrite <- H1.
+      apply (H a); left; reflexivity.
+      assert (forall x:json, In x c -> json_normalized (normalize_json x))
+        by (intros; apply (H x0); right; assumption).
+      specialize (IHc H2 H1).
+      assumption.
+    - apply jnobject.
+      + apply Forall_sorted.
+        apply Forall_forall; intros.
+        induction r.
+        contradiction.
+        simpl in *.
+        elim H0; intros; clear H0.
+        rewrite <- H1.
+        simpl.
+        apply (H (fst a) (snd a)).
+        left; destruct a; reflexivity.
+        assert (forall (x : string) (y : json),
+                   In (x, y) r -> json_normalized (normalize_json y)); intros.
+        apply (H x0 y); right; assumption.
+        apply (IHr H0).
+        assumption.
+      + apply (@rec_sort_sorted string ODT_string) with (l1 := (map (fun x : string * json => (fst x, normalize_json (snd x))) r)).
+        reflexivity.
+  Qed.
+
+  Theorem normalize_normalized_eq {d}:
+    json_normalized d ->
+    normalize_json d = d.
+  Proof.
+    induction d using jsonInd2; simpl; trivial.
+    - intros.
+      rewrite (@map_eq _ _ normalize_json id).
+      + rewrite map_id; trivial.
+      + inversion H0; simpl; subst.
+        revert H2. apply Forall_impl_in.
+        auto.
+    - intros.
+      inversion H0; subst.
+      rewrite (@map_eq _ _ (fun x : string * json => (fst x, normalize_json (snd x))) id).
+      + rewrite map_id.
+        rewrite rec_sorted_id; trivial.
+      + revert H2. apply Forall_impl_in.
+        destruct a; unfold id; simpl; intros.
+        f_equal; eauto.
+  Qed.
+
+  Lemma map_normalize_normalized_eq c :
+    Forall (fun x => json_normalized (snd x)) c ->
+    (map
+       (fun x0 : string * json => (fst x0, normalize_json (snd x0)))
+       c) = c.
+  Proof.
+    induction c; simpl; trivial.
+    destruct a; inversion 1; simpl in *; subst.
+    rewrite normalize_normalized_eq; trivial.
+    rewrite IHc; trivial.
+  Qed.
+
+
+  Corollary normalize_idem d :
+    normalize_json (normalize_json d) = normalize_json d.
+  Proof.
+    apply normalize_normalized_eq.
+    apply normalize_normalizes.
+  Qed.
+
+  Corollary normalize_json_eq_normalized {d} :
+    normalize_json d = d -> json_normalized d.
+  Proof.
+    intros.
+    generalize (normalize_normalizes d).
+    congruence.
+  Qed.
+  
+  Theorem normalized_json_dec d : {json_normalized d} + {~ json_normalized d}.
+  Proof.
+    destruct (normalize_json d == d); unfold equiv, complement in *.
+    - left. apply normalize_json_eq_normalized; trivial.
+    - right. intro dn; elim c. apply normalize_normalized_eq; trivial.
+  Defined.
+
+  Lemma json_normalized_jarray a l :
+    (json_normalized a /\ json_normalized (jarray l)) <->
+    json_normalized (jarray (a :: l)).
+  Proof.
+    split.
+    - destruct 1 as [d1 d2]. inversion d2; subst.
+      constructor; auto.
+    - inversion 1; subst. inversion H1; subst.
+      split; trivial.
+      constructor; auto.
+  Qed.
+  
+  Lemma json_normalized_rec_sort_app l1 l2 :
+    json_normalized (jobject l1) ->
+    json_normalized (jobject l2) ->
+    json_normalized (jobject (rec_sort (l1 ++ l2))).
+  Proof.
+    inversion 1; inversion 1; subst.
+    constructor; eauto 1.
+    apply Forall_sorted.
+    apply Forall_app; trivial.
+  Qed.
+
+  Lemma json_normalized_rec_concat_sort l1 l2 :
+    json_normalized (jobject l1) ->
+    json_normalized (jobject l2) ->
+    json_normalized (jobject (rec_concat_sort l1 l2)).
+  Proof.
+    apply json_normalized_rec_sort_app.
+  Qed.
+
+  Lemma json_normalized_jarray_in x l :
+    In x l ->
+    json_normalized (jarray l) ->
+    json_normalized x.
+  Proof.
+    inversion 2; subst.
+    rewrite Forall_forall in H2.
+    eauto.
+  Qed.
+
+  Lemma jnobject_nil : json_normalized (jobject nil).
+  Proof.
+    econstructor; trivial.
+  Qed.
+
+  Lemma jnobject_sort_content c :
+    Forall (fun d : string * json => json_normalized (snd d)) c ->
+    Forall (fun d : string * json => json_normalized (snd d)) (rec_sort c).
+  Proof.
+    intros F.
+    apply Forall_sorted; trivial.
+  Qed.
+
+  Lemma jnobject_sort c :
+    Forall (fun d : string * json => json_normalized (snd d)) c ->
+    json_normalized (jobject (rec_sort c)).
+  Proof.
+    intros F; econstructor; trivial.
+    apply Forall_sorted; trivial.
+  Qed.
+
+  Lemma json_normalized_jarray_Forall l :
+    json_normalized (jarray l) <-> Forall json_normalized l.
+  Proof.
+    split; intros H.
+    - invcs H; trivial.
+    - constructor; trivial.
+  Qed.
+  
+End JSONNorm.
+
